state theorem to prove body

arithmetic/Verif_arithmetic.v
@@ -5,16 +5,34 @@ Require Import Didactica.arithmetic.
 #[export] Instance CompSpecs : compspecs. make_compspecs prog. Defined.
 Definition Vprog : varspecs.  mk_varspecs prog. Defined.
 
-Definition t_number := Tstruct _number noattr.
+Definition struct_number := Tstruct _number noattr.
 
 (* For some reason coq has trouble typechecking this if it's inlined *)
-Definition make_number (l : list Z) (v : val) : reptype t_number :=
+Definition make_number (l : list Z) (v : val) : reptype struct_number :=
   ((Vint (Int.repr (Zlength l))), v).
 
 Definition cnumber {CS : compspecs} (sh : Share.t) (digit_list : list Z) (p : val) :=
   EX digits : val,
-  data_at Ews t_number (make_number digit_list digits) p *
+  data_at Ews struct_number (make_number digit_list digits) p *
   data_at sh (tarray tulong (Zlength digit_list)) (map Vint (map Int.repr digit_list)) digits.
+
+Lemma cnumber_local_facts:
+  forall sh digit_list p,
+   cnumber sh digit_list p |--
+   !! (isptr p).
+Proof.
+  intros. unfold cnumber. Intros digits. entailer!.
+Qed.
+
+Lemma cnumber_valid_pointer:
+  forall sh digit_list p,
+   cnumber sh digit_list p |-- valid_pointer p.
+Proof.
+  intros. unfold cnumber. Intros digits. entailer!.
+Qed.
+
+#[export] Hint Resolve cnumber_local_facts : saturate_local.
+#[export] Hint Resolve cnumber_valid_pointer : valid_pointer.
 
 Definition comparison_int c : val :=
   match c with
@@ -26,7 +44,7 @@ Definition comparison_int c : val :=
 Definition number_compare_spec : ident * funspec :=
  DECLARE _number_compare
   WITH sh0: share, sh1: share, n0 : val, n1 : val, d0 : list Z, d1 : list Z
-  PRE [ tptr t_number, tptr t_number ]
+  PRE [ tptr struct_number, tptr struct_number ]
     PROP (readable_share sh0; readable_share sh1)
     PARAMS (n0; n1)
     SEP (cnumber sh0 d0 n0 * cnumber sh1 d1 n1)
@@ -36,3 +54,8 @@ Definition number_compare_spec : ident * funspec :=
     SEP (cnumber sh0 d0 n0 * cnumber sh1 d1 n1).
 
 Definition Gprog : funspecs := [ number_compare_spec ].
+
+Lemma body_number_compare: semax_body Vprog Gprog f_number_compare number_compare_spec.
+Proof.
+  start_function.
+Admitted.
